ArithExpr.v
@@ -1,0 +1,254 @@
+(* v0.0.1 *)
+From Stdlib Require Import List.
+Import ListNotations.
+From TAPL Require Import Tactics RelationProp.
+
+Module NumberBoolean.
+
+(* Syntax *)
+Inductive tm: Type :=
+  | tm_true 
+  | tm_false 
+  | tm_if (t1: tm) (t2: tm) (t3: tm)
+  | tm_zero
+  | tm_succ (t: tm)
+  | tm_pred (t: tm)
+  | tm_iszero (t: tm).
+
+Inductive bv: tm -> Prop :=
+  | bv_true: bv tm_true
+  | bv_false: bv tm_false.
+
+Inductive nv: tm -> Prop :=
+  | nv_zero: nv tm_zero
+  | nv_succ: forall t, nv t -> nv (tm_succ t).
+
+Inductive value: tm -> Prop :=
+  | v_true: value tm_true
+  | v_false: value tm_false
+  | v_num: forall t, nv t -> value t.
+
+(* Evaluation *)
+(* SmallStep Semantics *)
+Reserved Notation "e '-->' n" (at level 90, left associativity).
+Inductive step: tm -> tm -> Prop :=
+  | E_IfTrue (t2 t3: tm): tm_if tm_true t2 t3 --> t2
+  | E_IfFalse (t2 t3: tm): tm_if tm_false t2 t3 --> t3
+  | E_If (t1 t1' t2 t3: tm): 
+    (t1 --> t1') -> (tm_if t1 t2 t3 --> tm_if t1' t2 t3)
+  | E_Succ (t t': tm):
+    (t --> t') -> (tm_succ t --> tm_succ t')
+  | E_PredZero: tm_pred tm_zero --> tm_zero
+  | E_PredSucc (t: tm):
+    nv t -> (tm_pred (tm_succ t) --> t)
+  | E_Pred (t t': tm):
+    (t --> t') -> (tm_pred t --> tm_pred t')
+  | E_IszeroZero: tm_iszero tm_zero --> tm_true
+  | E_IszeroSucc (t: tm):
+    nv t -> (tm_iszero (tm_succ t) --> tm_false)
+  | E_Iszero (t t': tm):
+    (t --> t') -> (tm_iszero t --> tm_iszero t')
+where "e '-->' n" := (step e n) : type_scope.
+
+Lemma bvalue_is_normal_form: forall t,
+bv t -> normal_form step t.
+Proof.
+  intros t Hbv. unfold normal_form.
+  induction Hbv.
+  - (* bv_true *) intros [t' Hstep]. inv Hstep.
+  - (* bv_false *) intros [t' Hstep]. inv Hstep.
+Qed.
+
+Lemma nvalue_is_normal_form: forall t,
+nv t -> normal_form step t.
+Proof.
+  intros t Hnv. unfold normal_form.
+  induction Hnv.
+  - (* nv_zero *) intros [t' Hstep]. inv Hstep.
+  - (* nv_succ *) intros [t' Hstep]. inv Hstep; try (inv H).
+    + (* E_PredSucc *) apply IHHnv. exists t'0. assumption.
+Qed.
+
+Lemma value_is_normal_form: forall t,
+value t -> normal_form step t.
+Proof.
+  intros t Hval. unfold normal_form.
+  destruct Hval.
+  - (* v_true *) apply bvalue_is_normal_form. apply bv_true.
+  - (* v_false *) apply bvalue_is_normal_form. apply bv_false.
+  - (* v_num *) apply nvalue_is_normal_form. assumption.
+Qed.
+
+(* Deterministic of small step *)
+(* if t-->t' /\ t-->t'' then t' = t'' *)
+Theorem step_deterministic:
+  deterministic step.
+Proof.
+  unfold deterministic.
+  intros x y1 y2 Hy1 Hy2.
+  generalize dependent y2.
+  induction Hy1.
+  - (* E_IfTrue *) intros. inv Hy2.
+    + reflexivity.
+    + inv H3.
+  - (* E_IfFalse *) intros. inv Hy2.
+    + reflexivity.
+    + inv H3.
+  - (* E_If *) intros. inv Hy2.
+    + inv Hy1.
+    + inv Hy1.
+    + f_equal. apply IHHy1. assumption.
+  - (* E_Succ *) intros. inv Hy2. f_equal. apply IHHy1. assumption.
+  - (* E_PredZero *) intros. inv Hy2.
+    + reflexivity.
+    + inv H0.
+  - (* E_PredSucc *) intros. inv Hy2.
+    + reflexivity.
+    + inv H1.  
+Admitted.
+
+Notation " t '-->*' t' " := (multi step t t') (at level 40).
+Example test_multi_step:
+  tm_if (tm_if tm_true tm_false tm_true) tm_true tm_false -->* tm_false.
+Proof.
+  apply multi_step with (y := tm_if tm_false tm_true tm_false).
+  - apply E_If. apply E_IfTrue.
+  - apply multi_step with (y := tm_false).
+    + apply E_IfFalse.
+    + apply multi_refl.
+Qed.
+
+(* Big Step Semantics *)
+Reserved Notation "e '==>' n" (at level 90, left associativity).
+Inductive tevalR: tm -> tm -> Prop :=
+  | B_Val (t: tm):
+      value t -> (t ==> t)
+  | B_IfTrue (t1 t2 t3 t2': tm):
+      (value t2) ->
+      (t1 ==> tm_true) ->
+      (t2 ==> t2') ->
+      (tm_if t1 t2 t3 ==> t2')
+  | B_IfFalse (t1 t2 t3 t3': tm):
+      (value t3) ->
+      (t1 ==> tm_false) ->
+      (t3 ==> t3') ->
+      (tm_if t1 t2 t3 ==> t3')
+  | B_Succ (t t' : tm):
+      (nv t') ->
+      (t ==> t') ->
+      (tm_succ t ==> tm_succ t')
+  | B_PredZero (t: tm):
+      (t ==> tm_zero) ->
+      (tm_pred t ==> tm_zero)
+  | B_PredSucc (t t' : tm):
+      (nv t') ->
+      (t ==> tm_succ t') ->
+      (tm_pred t ==> t')
+  | B_IszeroZero (t: tm):
+      (t ==> tm_zero) ->
+      (tm_iszero t ==> tm_true)
+  | B_IszeroSucc (t t' : tm):
+      (nv t') ->
+      (t ==> tm_succ t') ->
+      (tm_iszero t ==> tm_false)
+where "e '==>' n" := (tevalR e n) : type_scope.
+
+Lemma step_eval: forall t t' v,
+  (value v) -> (t --> t') -> (t' ==> v) -> (t ==> v).
+Proof.
+  auto.
+Admitted.
+
+Theorem coinsident_eval:
+  forall t t', (value t') ->
+  (t -->* t') <-> (t ==> t').
+Proof.
+  intros t t'. split.
+  - (* t -->* t' -> t ==> t' *)
+    intros Hmulti. induction Hmulti.
+    + (* multi_refl *) apply B_Val. assumption.
+    + (* multi_step *) destruct H0 eqn:E.
+      * (* E_IfTrue *) apply B_IfTrue. 
+Admitted.
+
+Lemma nf_multi_btstep :
+  forall t1 t2,
+  normal_form btstep t1 ->
+  t1 -->* t2 ->
+  t1 = t2.
+Proof.
+  intros t1 t2 Hnf Hmulti.
+  induction Hmulti.
+  - (* multi_refl *) reflexivity.
+  - (* multi_step *) unfold normal_form in Hnf. exfalso. apply Hnf. exists t2. exact H.
+Qed.
+
+Theorem unique_normal_forms :
+  forall t t1 t2,
+  t -->* t1 ->
+  normal_form btstep t1 ->
+  t -->* t2 ->
+  normal_form btstep t2 ->
+  t1 = t2.
+Proof.
+  intros t t1 t2 Hmulti1 Hnf1 Hmulti2 Hnf2.
+  induction Hmulti1.
+  - (* multi_refl *)
+    apply nf_multi_btstep with (t1 := t) (t2 := t2).
+    exact Hnf1.
+    exact Hmulti2.
+  - (* multi_step *)
+
+Lemma multi_btstep_If : forall t1 t1' t2 t3,
+t1 -->* t1' ->
+BTIf t1 t2 t3 -->* BTIf t1' t2 t3.
+Proof.
+  intros t1 t1' t2 t3 Hmulti.
+  induction Hmulti. 
+  - (* multi_refl *)
+    apply multi_refl.
+  - (* multi_step *)
+    eapply multi_step.
+    eapply ST_If. exact H. exact IHHmulti.
+Qed.
+
+Example btstep_If_true_normalizing : forall t1 t2 t3, exists t', (t1 -->* BTTrue) -> (BTIf t1 t2 t3) -->* t'.
+Proof.
+  intros t1 t2 t3. eexists.
+  apply multi_btstep_If.
+Qed.
+
+Example btstep_If_false_normalizing : forall t1 t2 t3, exists t', (t1 -->* BTFalse) -> (BTIf t1 t2 t3) -->* t'.
+Proof.
+  intros t1 t2 t3. eexists.
+  apply multi_btstep_If.
+Qed.
+
+Theorem btstep_normarlizing:
+  forall t: bterm, exists t',
+  (t -->* t') /\ normal_form btstep t'.
+Proof.
+  intros t.
+  induction t.
+  - exists BTTrue. split.
+    + apply multi_refl.
+    + unfold normal_form. intros [t' Hstep]. inv Hstep.
+  - exists BTFalse. split.
+    + apply multi_refl.
+    + unfold normal_form. intros [t' Hstep]. inv Hstep.
+  - destruct IHt1 as [t1' [Hmulti1 Hnf1]].
+    destruct IHt2 as [t2' [Hmulti2 Hnf2]].
+    destruct IHt3 as [t3' [Hmulti3 Hnf3]].
+    destruct (nf_same_as_value t1') as [Hval1 _].
+    destruct (nf_same_as_value t2') as [Hval2 _].
+    destruct (nf_same_as_value t3') as [Hval3 _].
+    apply Hval1 in Hnf1. apply Hval2 in Hnf2. apply Hval3 in Hnf3.
+    clear Hval1 Hval2 Hval3.
+    inv Hnf1; inv Hnf2; inv Hnf3.
+    + (* t1' = BTTrue *) eexists. split.
+Admitted.
+
+End NumberBoolean.
+
+
+
