Props/RelationProp.v
@@ -1,0 +1,37 @@
+(* relation *)
+Definition relation (X Y: Type) := X -> Y -> Prop.
+
+(* deterministic on relation *)
+Definition deterministic {X Y: Type} (R: relation X Y): Prop :=
+  forall x y1 y2, R x y1 -> R x y2 -> y1 = y2.
+
+Definition normal_form {X Y : Type}
+(R : relation X Y) (t : X) : Prop :=
+~ exists t', R t t'.
+
+(* multi_step on Self Relation *)
+Inductive multi {X: Type} (R : relation X X):relation X X :=
+  | multi_refl : forall (x : X), multi R x x
+  | multi_step : forall (x y z : X), R x y -> multi R y z -> multi R x z.
+
+Theorem multi_R : forall (X : Type) (R : relation X X) (x y : X),
+R x y -> (multi R) x y.
+Proof.
+  intros X R x y H.
+  apply multi_step with (y := y).
+  - exact H.
+  - apply multi_refl.
+Qed.
+
+Theorem multi_trans :
+  forall (X : Type) (R : relation X X) (x y z : X),
+  (multi R) x y -> (multi R) y z -> (multi R) x z.
+Proof.
+  intros X R x y z Hxy Hyz.
+  induction Hxy.
+  - exact Hyz.
+  - apply IHHxy in Hyz.
+    apply multi_step with (y := y).
+    + exact H.
+    + exact Hyz.
+Qed.
